Uppaal_Networks/UPPAAL_Asm_Test.thy
@@ -182,23 +182,6 @@ definition "dumb_result \<equiv>
 
 value "sorted_list_of_set (domain dumb_entry)"
 
-(* *)
-
-(* TODO: Where does the enum dependency come from? *)
-(*instantiation dumb_base :: enum
-begin
-  definition "enum_dumb_base \<equiv> [Any]"
-  definition "enum_all_dumb_base (f::dumb_base \<Rightarrow> bool) = True"
-  definition "enum_ex_dumb_base (f::dumb_base \<Rightarrow> bool) = True"
-  instance sorry
-end*)
-
-lemma[code_unfold]: "(a::dumb) = \<bottom> \<equiv> (case a of None \<Rightarrow> True | _ \<Rightarrow> False)"
-  by (smt bot_option_def option.case_eq_if)
-
-export_code step_map dumb_step spprog dumb_entry mysprog in Haskell module_name Test
-
-(*declare [[ML_source_trace]]*)
 value "dumb_stepped"
 definition "abs_res_str \<equiv> String.implode (show (DisplayCtx mysprog dumb_stepped))"
 ML \<open>val _ = writeln (@{code abs_res_str})\<close>
